refactoring

test/RReals.v
@@ -1,44 +1,43 @@
 From Coq Require Import Lia Arith.PeanoNat Classical_Prop.
-From Mecha Require Import Resource Term Cell.
-From Mecha Require ET_Definition ET_Props.
+From Mecha Require Import Resource Term RReal Evaluation RReal.
 From DeBrLevel Require Import LevelInterface MapLevelInterface MapLevel MapExtInterface 
                MapExt.
 From MMaps Require Import MMaps.
 
 
 (** * Environment between resources and cells *)
-Module REnvironment <: IsLvlET.
-Include MapLvlD.MakeLvlMapWLLVL Cell.
+Module RReals <: IsLvlET.
+Include MapLvlD.MakeLvlMapWLLVL RReal.
 
 Import Raw Ext.
 
 (** *** Definition *)
-
+(*
 Definition embeds_func V v := 
     add (new_key V) ([⧐ᵣₓ (new_key V) ≤ 1 ] ⩽ v … ⩾) (shift (new_key V) 1 V).
 
 Definition embeds_func_revert v V := embeds_func V v. 
 
-Definition embeds_gen (V : REnvironment.t) (l : list Λ) := 
+Definition embeds_gen (V : RReals.t) (l : list Λ) := 
   List.fold_left embeds_func l V.
 
-Definition For_all (P : resource -> Cell.t -> Prop) (V : REnvironment.t) := 
+Definition For_all (P : resource -> RReal.t -> Prop) (V : RReals.t) := 
   forall r v, find r V = Some v -> P r v. 
 
 Definition embeds := embeds_gen empty. 
 
-Definition extracts (V : REnvironment.t) : list (option Λ) :=
+Definition extracts (V : RReals.t) : list (option Λ) :=
   List.map (fun x =>  match (find x V) with
                         | Some (⩽ … v ⩾) => Some v
                         | Some _ => None
                         | None   => None
                       end) (seq 0 (max_key V)).
 
-Definition halts (k : Lvl.t) (V : REnvironment.t) := forall (r : resource) (v : 𝑣), 
- find r V = Some v -> ET_Definition.halts k (Cell.extract v).
+Definition halts (k : Lvl.t) (V : RReals.t) := forall (r : resource) (v : 𝑣), 
+ find r V = Some v -> halts k (RReal.extract v).
 
-Definition used r (V : REnvironment.t) := exists v, find r V = Some (⩽ … v ⩾).
-Definition unused r (V : REnvironment.t) := exists v, find r V = Some (⩽ v … ⩾).
+Definition used r (V : RReals.t) := exists v, find r V = Some (⩽ … v ⩾).
+Definition unused r (V : RReals.t) := exists v, find r V = Some (⩽ v … ⩾).
 
 (** *** Embedding *)
 
@@ -131,8 +130,8 @@ Proof.
 Qed.
 
 Lemma embedding_Forall_unused : forall l V,
-  For_all (fun _ v => Cell.unused v) V ->
-  For_all (fun _ v => Cell.unused v) (embeds_gen V l).
+  For_all (fun _ v => RReal.unused v) V ->
+  For_all (fun _ v => RReal.unused v) (embeds_gen V l).
 Proof.
   unfold For_all; intros. assert (In r (embeds_gen V l)).
   { exists v; now apply find_2. }
@@ -157,20 +156,20 @@ Proof.
   - split. 
     -- unfold Resource.valid; lia.
     -- split.
-      * apply Cell.valid_weakening with (k := new_key m); auto.
+      * apply RReal.valid_weakening with (k := new_key m); auto.
       * apply valid_add_notin_spec.
         ** apply new_key_notin_spec; lia.
         ** split.
             + unfold Resource.valid; lia.
             + split.
-              ++ apply Cell.valid_weakening with (k := new_key m); auto.
+              ++ apply RReal.valid_weakening with (k := new_key m); auto.
               ++ apply valid_weakening with (k := new_key m); auto.
 Qed.
 
 Lemma valid_wh_spec_1 : forall m v v',
   valid (new_key m) m -> (new_key m) ⊩ᵣₓ v -> (new_key m) ⊩ᵣₓ v' -> 
   valid (S (S (new_key m))) (add (S (new_key m)) v 
-                              (add (new_key m) (Cell.shift (new_key m) 2 v') (shift (new_key m) 2 m))).
+                              (add (new_key m) (RReal.shift (new_key m) 2 v') (shift (new_key m) 2 m))).
 Proof.
   intros. apply valid_add_notin_spec.
   - apply new_key_notin_spec; rewrite new_key_add_spec_1; auto.
@@ -178,19 +177,19 @@ Proof.
     * rewrite shift_new_spec; auto.
   - repeat split. 
     -- unfold Resource.valid; lia.
-    -- apply Cell.valid_weakening with (k := new_key m); auto.
+    -- apply RReal.valid_weakening with (k := new_key m); auto.
     -- apply valid_add_notin_spec.
        * apply new_key_notin_spec; auto; rewrite shift_new_spec; auto.
        * repeat split.
          + unfold Resource.valid; lia.
          + replace (S (S (new_key m))) with ((new_key m) + 2) by lia. 
-           now apply Cell.shift_preserves_valid_1.
+           now apply RReal.shift_preserves_valid_1.
          + replace (S (S (new_key m))) with ((new_key m) + 2) by lia. 
            now apply shift_preserves_valid_1.  
 Qed.
 
 Lemma valid_update_spec : forall m r v k,
-  In r m -> valid k m -> Cell.valid k v -> valid k (add r v m).
+  In r m -> valid k m -> RReal.valid k v -> valid k (add r v m).
 Proof.
   intro m; induction m using map_induction; intros r v k HIn Hvm Hvv.
   - unfold Empty in *; exfalso.
@@ -279,7 +278,7 @@ Qed.
 
 Lemma shift_find_e_spec_1 : forall lb k r v V,
   find r (shift lb k V) = Some v -> 
-  (exists r', r = ([⧐ᵣ lb ≤ k] r')) /\ exists v', Cell.eq v (Cell.shift lb k v').
+  (exists r', r = ([⧐ᵣ lb ≤ k] r')) /\ exists v', RReal.eq v (RReal.shift lb k v').
 Proof.
   intros.
   assert (In r (shift lb k V)). { now exists v; apply find_2. }
@@ -293,7 +292,7 @@ Qed.
 (** *** Halts *)
 
 Lemma halts_add_spec : forall m k x v,
-  (ET_Definition.halts k (Cell.extract v)) /\ halts k m -> halts k (add x v m).
+  (Evaluation.halts k (RReal.extract v)) /\ halts k m -> halts k (add x v m).
 Proof.
   intros m k x v [Hltv Hltm]; unfold halts; intros r v' Hfi.
   rewrite add_o in Hfi; destruct (Resource.eq_dec x r); subst; inversion Hfi; subst; auto.
@@ -306,7 +305,7 @@ Proof.
   apply shift_find_e_spec_1 in HfV as HI. destruct HI as [[r' Heqr'] [v' Heqv']]; subst.
   rewrite Heqv' in *; clear Heqv'; rewrite <- shift_find_spec in HfV.
   apply Hlt in HfV.
-  destruct v,v'; simpl in *; apply ET_Props.halts_weakening; auto.
+  destruct v,v'; simpl in *; apply Evaluation.halts_weakening; auto.
 Qed.
 
 Lemma halts_weakening_1 : 
@@ -329,7 +328,7 @@ Qed.
 
 Lemma new_key_wh_spec m v v' :
   new_key (add (S (new_key m)) v 
-          (add (new_key m) (Cell.shift (new_key m) 2 v') 
+          (add (new_key m) (RReal.shift (new_key m) 2 v') 
                                       (shift (new_key m) 2 m))) = S (S (new_key m)).
 Proof.
   rewrite new_key_add_spec_1; auto.
@@ -342,9 +341,10 @@ Proof.
 Qed.
 
 (** *** Morphism *)
+*)
 
 #[global] 
-Instance in_renv : 
+Instance in_rreals : 
   Proper (Logic.eq ==> eq ==> iff) In.
 Proof.
   repeat red; intros; split; intros;
@@ -353,128 +353,127 @@ Proof.
 Qed.
 
 #[global] 
-Instance find_renv : Proper (Logic.eq ==> eq ==> Logic.eq) find.
+Instance find_rreals : Proper (Logic.eq ==> eq ==> Logic.eq) find.
 Proof. repeat red; intros; subst. now rewrite H0. Qed.
 
 #[global] 
-Instance Empty_renv : Proper (eq ==> iff) Empty.
+Instance Empty_rreals : Proper (eq ==> iff) Empty.
 Proof. red; red; intros; now apply Empty_eq_spec. Qed.
 
 #[export] 
-Instance Add_renv : 
-Proper (Resource.eq ==> Cell.eq ==> eq ==> eq ==> iff) (@Add Cell.t).
+Instance Add_rreals : 
+Proper (Resource.eq ==> RReal.eq ==> eq ==> eq ==> iff) (@Add RReal.t).
 Proof. 
-  red; red; red; red; red; intros. apply Cell.eq_leibniz in H0; subst.
+  red; red; red; red; red; intros. apply RReal.eq_leibniz in H0; subst.
   rewrite H. unfold Add in *. rewrite H1; rewrite H2. split; intros; auto.
 Qed.
 
 #[global] 
-Instance add_renv : 
-Proper (Resource.eq ==> Cell.eq ==> REnvironment.eq ==> REnvironment.eq) 
-                                                          (@add Cell.t).
+Instance add_rreals : 
+Proper (Resource.eq ==> RReal.eq ==> RReals.eq ==> RReals.eq) 
+                                                          (@add RReal.t).
 Proof. 
- red; red; red; red; red; intros; subst; apply Cell.eq_leibniz in H0; subst.
+ red; red; red; red; red; intros; subst; apply RReal.eq_leibniz in H0; subst.
  rewrite H1; now rewrite H. 
 Qed. 
 
 #[global] 
 Instance Submap_env : 
-  Proper (REnvironment.eq ==> REnvironment.eq ==> iff) REnvironment.Submap.
+  Proper (RReals.eq ==> RReals.eq ==> iff) RReals.Submap.
 Proof. 
   repeat red; intros; split; intros.
-  - rewrite REnvironment.Submap_eq_left_spec in H1; eauto.
-    rewrite REnvironment.Submap_eq_right_spec in H1; eauto.
-  - rewrite <- REnvironment.Submap_eq_left_spec in H1; eauto.
-    rewrite <- REnvironment.Submap_eq_right_spec in H1; eauto.
+  - rewrite RReals.Submap_eq_left_spec in H1; eauto.
+    rewrite RReals.Submap_eq_right_spec in H1; eauto.
+  - rewrite <- RReals.Submap_eq_left_spec in H1; eauto.
+    rewrite <- RReals.Submap_eq_right_spec in H1; eauto.
 Qed.
 
-End REnvironment.
+End RReals.
 
 
 (** *** Scope and Notations *)
 
-Declare Scope renvironment_scope.
-Delimit Scope renvironment_scope with re.
+Declare Scope rreals_scope.
+Delimit Scope rreals_scope with rf.
 
-Definition 𝓥 := REnvironment.t.
+Definition 𝐅 := RReals.t.
 
-Infix "⊆ᵣᵦ" := REnvironment.Submap (at level 20, no associativity). 
-Infix "∈ᵣᵦ" := REnvironment.Raw.In (at level 20, no associativity). 
-Notation "r '∉ᵣᵦ' Re" := (~ (REnvironment.Raw.In r Re)) (at level 20, 
+Infix "⊆ᵣₔ" := RReals.Submap (at level 20, no associativity). 
+Infix "∈ᵣₔ" := RReals.Raw.In (at level 20, no associativity). 
+Notation "r '∉ᵣₔ' Re" := (~ (RReals.Raw.In r Re)) (at level 20, 
                                                                         no associativity). 
-Notation "∅ᵣᵦ" := REnvironment.Raw.empty (at level 20, no associativity). 
-Notation "'isEmptyᵣᵦ(' Re ')'" := (REnvironment.Empty Re) (at level 20, no associativity). 
-Notation "'Addᵣᵦ'" := (REnvironment.Add) (at level 20, no associativity). 
-Notation "R '⌊' x '⌋ᵣᵦ'"  := (REnvironment.Raw.find x R) (at level 15, x constr).
-Notation "'maxᵣᵦ(' R ')'"  := (REnvironment.Ext.max_key R) (at level 15).
-Notation "'newᵣᵦ(' R ')'"  := (REnvironment.Ext.new_key R) (at level 15).
-Notation "⌈ x ⤆ v '⌉ᵣᵦ' R"  := (REnvironment.Raw.add x v R) (at level 15, 
+Notation "∅ᵣₔ" := RReals.Raw.empty (at level 20, no associativity). 
+Notation "'isEmptyᵣₔ(' Re ')'" := (RReals.Empty Re) (at level 20, no associativity). 
+Notation "'Addᵣₔ'" := (RReals.Add) (at level 20, no associativity). 
+Notation "R '⌊' x '⌋ᵣₔ'"  := (RReals.Raw.find x R) (at level 15, x constr).
+Notation "'maxᵣₔ(' R ')'"  := (RReals.Ext.max_key R) (at level 15).
+Notation "⌈ x ⤆ v '⌉ᵣₔ' R"  := (RReals.Raw.add x v R) (at level 15, 
                                                                           x constr, v constr).
-Notation "R ⌈ x ⩦ v '⌉ᵣᵦ'"  := (REnvironment.Raw.find x R = Some v) (at level 15, 
+Notation "R ⌈ x ⩦ v '⌉ᵣₔ'"  := (RReals.Raw.find x R = Some v) (at level 15, 
                                                                                   x constr, 
                                                                                   v constr).
-Notation "R ⌈ x ⩦ ⊥ '⌉ᵣᵦ'"  := (REnvironment.Raw.find x R = None) (at level 15, 
+Notation "R ⌈ x ⩦ ⊥ '⌉ᵣₔ'"  := (RReals.Raw.find x R = None) (at level 15, 
                                                                                     x constr).
 
-Infix "=" := REnvironment.eq : renvironment_scope.
+Infix "=" := RReals.eq : rreals_scope.
 
-Notation "V '⁺ᵣᵦ'" := (REnvironment.Ext.new_key V) (at level 16).
+Notation "V '⁺ᵣₔ'" := (RReals.Ext.new_key V) (at level 16).
 
-Notation "'[⧐ᵣᵦ' lb '≤' k ']' t" := (REnvironment.shift lb k t) (at level 45, 
+Notation "'[⧐ᵣₔ' lb '≤' k ']' t" := (RReals.shift lb k t) (at level 45, 
                                                                       right associativity).
-Infix "⊩ᵣᵦ" := REnvironment.valid (at level 20, no associativity).
+Infix "⊩ᵣₔ" := RReals.valid (at level 20, no associativity).
 
 #[global]
-Instance eq_equiv_re : Equivalence REnvironment.eq.
-Proof. apply REnvironment.Equal_equiv. Qed.
+Instance eq_equiv_re : Equivalence RReals.eq.
+Proof. apply RReals.Equal_equiv. Qed.
 
-#[global] Instance max_renv : Proper (REnvironment.eq ==> Logic.eq) (REnvironment.Ext.max_key).
-          Proof. apply REnvironment.Ext.max_key_eq. Qed.
+#[global] Instance max_rreals : Proper (RReals.eq ==> Logic.eq) (RReals.Ext.max_key).
+          Proof. apply RReals.Ext.max_key_eq. Qed.
 
-#[global] Instance new_renv : Proper (REnvironment.eq ==> Logic.eq) (REnvironment.Ext.new_key).
-          Proof. apply REnvironment.Ext.new_key_eq. Qed.
-
-#[global] 
-Instance in_renv : 
-  Proper (Logic.eq ==> REnvironment.eq ==> iff) (REnvironment.Raw.In).
-Proof. apply REnvironment.in_renv. Qed.
+#[global] Instance new_rreals : Proper (RReals.eq ==> Logic.eq) (RReals.Ext.new_key).
+          Proof. apply RReals.Ext.new_key_eq. Qed.
 
 #[global] 
-Instance find_renv : Proper (Logic.eq ==> REnvironment.eq ==> Logic.eq) 
-                                                      (REnvironment.Raw.find).
-Proof. apply REnvironment.find_renv. Qed.
+Instance in_rreals : 
+  Proper (Logic.eq ==> RReals.eq ==> iff) (RReals.Raw.In).
+Proof. apply RReals.in_rreals. Qed.
 
 #[global] 
-Instance Empty_renv : Proper (REnvironment.eq ==> iff) (REnvironment.Empty).
-Proof. apply REnvironment.Empty_renv. Qed.
+Instance find_rreals : Proper (Logic.eq ==> RReals.eq ==> Logic.eq) 
+                                                      (RReals.Raw.find).
+Proof. apply RReals.find_rreals. Qed.
 
 #[global] 
-Instance Add_renv : 
-Proper (Resource.eq ==> Cell.eq ==> REnvironment.eq ==> REnvironment.eq ==> iff) 
-                                                  (@REnvironment.Add Cell.t).
-Proof. apply REnvironment.Add_renv. Qed. 
+Instance Empty_rreals : Proper (RReals.eq ==> iff) (RReals.Empty).
+Proof. apply RReals.Empty_rreals. Qed.
 
 #[global] 
-Instance add_renv : 
-Proper (Resource.eq ==> Cell.eq ==> REnvironment.eq ==> REnvironment.eq) 
-                                                          (@REnvironment.Raw.add Cell.t).
-Proof. apply REnvironment.add_renv. Qed. 
+Instance Add_rreals : 
+Proper (Resource.eq ==> RReal.eq ==> RReals.eq ==> RReals.eq ==> iff) 
+                                                  (@RReals.Add RReal.t).
+Proof. apply RReals.Add_rreals. Qed. 
+
+#[global] 
+Instance add_rreals : 
+Proper (Resource.eq ==> RReal.eq ==> RReals.eq ==> RReals.eq) 
+                                                          (@RReals.Raw.add RReal.t).
+Proof. apply RReals.add_rreals. Qed. 
 
 #[global] 
 Instance Submap_env : 
-  Proper (REnvironment.eq ==> REnvironment.eq ==> iff) REnvironment.Submap.
-Proof. apply REnvironment.Submap_env. Qed.
+  Proper (RReals.eq ==> RReals.eq ==> iff) RReals.Submap.
+Proof. apply RReals.Submap_env. Qed.
 
 #[global] 
-Instance Submap_env_po : PreOrder REnvironment.Submap.
-Proof. apply REnvironment.Submap_po. Qed. 
+Instance Submap_env_po : PreOrder RReals.Submap.
+Proof. apply RReals.Submap_po. Qed. 
 
 #[global] 
-Instance valid_renv : Proper (Logic.eq ==> REnvironment.eq ==> iff) REnvironment.valid.
-Proof. apply REnvironment.valid_eq. Qed.
+Instance valid_rreals : Proper (Logic.eq ==> RReals.eq ==> iff) RReals.valid.
+Proof. apply RReals.valid_eq. Qed.
 
 #[global] 
-Instance shift_renv : 
-  Proper (Logic.eq ==> Logic.eq ==> REnvironment.eq ==> REnvironment.eq) REnvironment.shift.
-Proof. apply REnvironment.shift_eq. Qed.
+Instance shift_rreals : 
+  Proper (Logic.eq ==> Logic.eq ==> RReals.eq ==> RReals.eq) RReals.shift.
+Proof. apply RReals.shift_eq. Qed.
 
