theories/Syntax/Resource.v
@@ -1,3 +1,4 @@
+From Coq Require Import Lia PeanoNat.
 From DeBrLevel Require Import LevelInterface Level PairLevel.
 
 (** * Syntax - Resource
@@ -6,7 +7,42 @@ From DeBrLevel Require Import LevelInterface Level PairLevel.
   we need identifiers for resources. Thus, we choose De Bruijn level as representation in
   order to avoid capture variables. It is a direct use of the [Level] module.
 *)
-Module Resource <: IsBdlLvlFullOTWL := Level.
+Module Resource <: IsBdlLvlFullOTWL.
+
+Include Level.
+
+Definition multi_shift (lbs : list nat) (ks : list nat) (t : t) :=
+  List.fold_right (fun (x : nat * nat) acc => let (lb,k) := x in shift lb k acc) t (List.combine lbs ks).
+
+Lemma shift_unfold_2 lb lb' k k' r:
+  lb' <= lb -> lb' <= k' -> lb <= k' -> 
+  shift lb k (shift lb' (k' - lb') r) = shift lb' (k + (k' - lb')) r.
+Proof.
+  intros.
+  unfold shift; destruct (Nat.leb_spec0 lb' r).
+  - replace (lb <=? r + (k' - lb')) with true; try lia.
+    symmetry. apply Nat.leb_le. lia.
+  - replace (lb <=? r) with false; auto.
+    symmetry. apply Nat.leb_nle; lia.
+Qed.
+
+Lemma multi_shift_valid_refl lbs ks lb t:
+  valid lb t -> (forall i, List.In i lbs -> lb <= i) ->
+  multi_shift lbs ks t = t.
+Proof.
+  revert ks lb t. induction lbs.
+  - intros; unfold multi_shift; now simpl in *.
+  - intros; unfold multi_shift in *; destruct ks; simpl; auto.
+    rewrite IHlbs with (lb := lb); auto.
+    -- rewrite shift_valid_refl; auto.
+       unfold valid in *.
+       assert (lb <= a). { apply H0; simpl; now left. }
+       lia.
+    -- intros. apply H0; simpl; now right.
+Qed.
+
+
+End Resource.
 
 (** * Syntax - Pair of resources *)
 Module PairResource <: IsBdlLvlFullETWL := IsBdlLvlFullPairOTWL Resource Resource.
@@ -30,6 +66,7 @@ Infix "=?" := Resource.eqb  (at level 70) : resource_scope.
 Infix "⊩ᵣ" := Resource.valid (at level 20, no associativity). 
 Infix "⊩?ᵣ" := Resource.validb (at level 20, no associativity). 
 Notation "'[⧐ᵣ' lb '≤' k ']' t" := (Resource.shift lb k t) (at level 65, right associativity).
+Notation "'[⧐⧐ᵣ' lb '≤' k ']' t" := (Resource.multi_shift lb k t) (at level 65, right associativity).
 
 Notation "'[⧐ₚᵣ' lb '≤' k ']' t" := (PairResource.shift lb k t) (in custom wormholes at level 45, 
                                                                             right associativity).
