theories/Transition/Functional/FT_Preservation.v
@@ -1,106 +1,10 @@
 From Coq Require Import Program Lia Relations.Relation_Definitions Classes.RelationClasses PeanoNat
                         Classical_Prop Classical_Pred_Type Bool.Bool Classes.Morphisms.
-From Mecha Require Import Resource Resources Term Typ Var ReadStock WriteStock
-               Substitution Typing VContext RContext Evaluation
-               Cell REnvironment Stock WfEnv.
-
-(** * Transition - Functional
-
-Wormholes's semantics are divided in three sub semantics:
-- evaluation transition
-- functional transition <--
-- temporal transition
-
-*)
+From Mecha Require Import Resource Resources Term Typ Var ReadStock WriteStock Typing VContext RContext ET_Definition
+                          Cell REnvironment Stock FT_Definition ET_Props ET_Preservation FT_Props.
 
 Module RC := RContext.
 Module RE := REnvironment.
-
-(** *** Definition *)
-
-Reserved Notation "⪡ V ; st ; t ⪢ ⭆ ⪡ V1 ; st1 ; t1 ; W ⪢" (at level 57, V constr, 
-                                                                V1 constr, st custom wormholes,
-                                                                st1 custom wormholes,
-                                                                t custom wormholes, 
-                                                                t1 custom wormholes, 
-                                                                no associativity).
-Reserved Notation "'Wfᵣₜ(' Re , V )" (at level 50).
-
-Inductive functional : 𝓥 -> Λ -> Λ -> 𝓥 -> Λ -> Λ -> 𝐖 -> Prop :=
-
-  | fT_eT_sf  :  forall (V V1 : 𝓥) (st st' t t' t'' : Λ) (W : 𝐖),
-
-        V⁺ᵣᵦ ⊨ t ⟼ t' -> ⪡ V ; st ; t' ⪢ ⭆ ⪡ V1 ; st' ; t'' ; W ⪢ -> 
-    (*-----------------------------------------------------------------------*)
-              ⪡ V ; st ; t ⪢ ⭆ ⪡ V1 ; st' ; t'' ; W ⪢
-
-  | fT_eT_sv  :  forall (V V1 : 𝓥) (st st' st'' t t' : Λ) (W : 𝐖),
-
-        V⁺ᵣᵦ ⊨ st ⟼ st' -> ⪡ V ; st' ; t ⪢ ⭆ ⪡ V1 ; st'' ; t' ; W ⪢ -> 
-    (*-----------------------------------------------------------------------*)
-              ⪡ V ; st ; t ⪢ ⭆ ⪡ V1 ; st'' ; t' ; W ⪢
-
-  | fT_arr   :  forall (st t : Λ) (V : 𝓥), 
-
-    (*---------------------------------------------------------*)
-        ⪡ V ; st ; arr(t) ⪢ ⭆ ⪡ V ; (t st) ; arr(t) ; ∅ₛₖ ⪢ 
-
-  | fT_first :  forall (v1 v1' v2 t t' : Λ) (τ : Τ) (V V1 : 𝓥) (W : 𝐖),
-
-        ⪡ V ; v1 ; t ⪢ ⭆ ⪡ V1 ; v1' ; t' ; W ⪢ ->
-    (*----------------------------------------------------------------------------------------*)
-        ⪡ V ; ⟨v1,v2⟩ ; first(τ:t) ⪢ 
-          ⭆ ⪡ V1 ; ⟨v1',[⧐ₜₘ {V⁺ᵣᵦ} ≤ {V1⁺ᵣᵦ - V⁺ᵣᵦ}] v2⟩ ; first(τ:t') ; W ⪢
-
-  | fT_comp  :  forall (st st' st'' t1 t1' t2 t2' : Λ) (V V1 V2 : 𝓥) (W W': 𝐖),
-
-                                         ⪡ V ; st ; t1 ⪢ ⭆ ⪡ V1 ; st' ; t1' ; W ⪢ ->
-        ⪡ V1 ; st' ; ([⧐ₜₘ {V⁺ᵣᵦ} ≤ {V1⁺ᵣᵦ - V⁺ᵣᵦ}] t2) ⪢ ⭆ ⪡ V2 ; st'' ; t2' ; W' ⪢ ->
-    (*---------------------------------------------------------------------------------------*)
-        ⪡ V ; st ; (t1 >>> t2) ⪢ 
-          ⭆ ⪡ V2 ; st'' ; (([⧐ₜₘ {V1⁺ᵣᵦ} ≤ {V2⁺ᵣᵦ - V1⁺ᵣᵦ}] t1') >>> t2')
-                          ; (([⧐ₛₖ V1⁺ᵣᵦ ≤ (V2⁺ᵣᵦ - V1⁺ᵣᵦ)] W) ∪ W')%sk ⪢
-
-  | fT_rsf   :  forall (V : 𝓥) (st v : Λ) (r : resource),
-
-                                V ⌈r ⩦ ⩽ v … ⩾⌉ᵣᵦ -> 
-    (*-----------------------------------------------------------------------*)
-        ⪡ V ; st ; rsf[r] ⪢ ⭆ ⪡ ⌈ r ⤆ ⩽ … st ⩾ ⌉ᵣᵦ V ; v ; rsf[r] ; ∅ₛₖ ⪢
-
-  | fT_wh    :  forall (V V1 : 𝓥) (st st' i t t' : Λ) (W : 𝐖),
-                
-        ⪡ (⌈S (V⁺ᵣᵦ) ⤆ ⩽ <[unit]> … ⩾⌉ᵣᵦ (⌈V⁺ᵣᵦ ⤆ [⧐ᵣₓ V⁺ᵣᵦ ≤ 2] ⩽ i … ⩾⌉ᵣᵦ ([⧐ᵣᵦ V⁺ᵣᵦ ≤ 2] V))) ; 
-            ([⧐ₜₘ {V⁺ᵣᵦ} ≤ 2] st) ; t ⪢ ⭆ ⪡ V1 ; st' ; t' ; W ⪢ ->
-    (*-----------------------------------------------------------------------------------------*)
-        ⪡ V ; st ; wormhole(i;t) ⪢ 
-          ⭆ ⪡ V1 ; st' ; t' ; ⌈V⁺ᵣᵦ ~ S (V⁺ᵣᵦ) ⤆ <[[⧐ₜₘ {V⁺ᵣᵦ} ≤ {V1⁺ᵣᵦ - V⁺ᵣᵦ}] i]>⌉ₛₖ W ⪢
-
-where "⪡ V ; st ; t ⪢ ⭆ ⪡ V1 ; st1 ; t1 ; W ⪢" := (functional V st t V1 st1 t1 W)
-.
-
-(** ** Lift of multiple evaluation transitions *)
-
-Lemma fT_MeT_sf (V V1 : 𝓥) (W : 𝐖) (st st' t t' t'' : Λ) :
-
-       V⁺ᵣᵦ ⊨ t ⟼⋆ t' -> ⪡ V ; st ; t' ⪢ ⭆ ⪡ V1 ; st' ; t'' ; W ⪢ -> 
-    (*-------------------------------------------------------------------*)
-                ⪡ V ; st ; t ⪢ ⭆ ⪡ V1 ; st' ; t'' ; W ⪢.
-Proof.
-  intro HmeT. apply multi_indexed in HmeT as [k HieT].
-  revert V V1 st st' t t' t'' HieT; induction k; intros; inversion HieT; subst; auto.
-  apply fT_eT_sf with (t' := y); auto. apply IHk with (t' := t'); auto.
-Qed.
-
-Lemma fT_MeT_sv (V V1 : 𝓥) (W : 𝐖) (st st' st'' t t' : Λ) :
-
-       V⁺ᵣᵦ ⊨ st ⟼⋆ st' -> ⪡ V ; st' ; t ⪢ ⭆ ⪡ V1 ; st'' ; t' ; W ⪢ -> 
-    (*--------------------------------------------------------------------*)
-                ⪡ V ; st ; t ⪢ ⭆ ⪡ V1 ; st'' ; t' ; W ⪢.
-Proof.
-  intro HmeT. apply multi_indexed in HmeT as [k HieT].
-  revert V V1 st st' st'' t t' HieT; induction k; intros; inversion HieT; subst; auto.
-  apply fT_eT_sv with (st' := y); auto. apply IHk with (st' := st'); auto.
-Qed.
 
 Section safety.
 
@@ -1033,8 +937,6 @@ Proof.
                 }
                 { rewrite RC.new_key_wh_spec; lia. }
 Qed.
-
-(** *** Some corollaries *)
 
 Corollary functional_preserves_wf_env_fT (Re : ℜ) (V V1 : 𝓥) (W : 𝐖) (sv sv' sf sf' : Λ) 
                                                                       (τ τ' : Τ) (R : resources):
