theories/Transition/Evaluation/ET_Props.v
@@ -1,0 +1,553 @@
+From Coq Require Import Classical_Prop Bool.Bool Lia Classes.RelationClasses Program.
+From Mecha Require Import Typ Resource Resources Term Var VContext RContext Typing ET_Definition.
+
+(** * Transition - Evaluation - Properties *)
+
+(** ** Substitution function *)
+
+(** *** Substitution regards of variables *)
+
+Lemma subst_afi_refl : forall t x lb k,
+  ~ isFV(x,t) -> forall v, <[ [x:= v ~ lb ≤ k] t ]> = t.
+Proof with eauto.
+  intros t; induction t; unfold not; intros x lb k afi v1; try (now simpl);
+  try (simpl; f_equal; now eauto).
+  - simpl. destruct (Var.eqb_spec x v); subst; auto; exfalso; apply afi; constructor.
+  - simpl; destruct (Var.eqb_spec x v); subst; auto.
+    f_equal; apply IHt; unfold not; intros; apply afi; now constructor.
+Qed.
+
+Lemma subst_closed_refl : forall t lb k,
+  clₜₘ(t) -> forall x t', <[ [x := t' ~ lb ≤ k] t ]> = t.
+Proof. intros. apply subst_afi_refl. apply H. Qed.
+
+Lemma subst_refl : forall v (x : variable) lb, <[[x := v ~ lb ≤ 0] x]> = v.
+Proof. intros v x lb; simpl; rewrite Var.eqb_refl; now apply Term.shift_refl. Qed.
+
+Lemma closed_subst_not_afi : forall t x v lb k,
+  clₜₘ(v) ->  ~ isFV(x,<[ [x := v ~ lb ≤ k] t ]>).
+Proof.
+  unfold Term.closed, not; intro t; induction t; intros x v1 lb k Hcl HFV; simpl;
+  try (inversion HFV; subst; now eauto); simpl in *;
+  try (destruct (Var.eqb_spec x v); subst; eauto).
+  - apply (Hcl v). rewrite Term.shift_afi_iff; eauto.
+  - inversion HFV; auto.
+  - inversion HFV; subst; eauto.
+  - inversion HFV; subst; eauto.
+Qed.
+
+Lemma subst_shadow : forall t' x t v lb k,
+  clₜₘ(v) -> <[[x := t ~ lb ≤ k] ([ x := v ~ lb ≤ k] t')]> = <[ [x := v ~ lb ≤ k] t' ]>.
+Proof. intros; eapply subst_afi_refl; apply closed_subst_not_afi; assumption. Qed.
+
+Lemma subst_permute : forall t x x1 v v1 lb k,
+  x <> x1 -> clₜₘ(v) -> clₜₘ(v1) ->
+  <[[x1 := v1 ~ lb ≤ k] ([ x := v ~ lb ≤ k] t)]> = <[[x := v ~ lb ≤ k] ([ x1 := v1 ~ lb ≤ k] t)]>.
+Proof.
+  intro t; induction t; intros; simpl; try (now reflexivity); try (f_equal; now auto).
+  - (* var *)
+    destruct (Var.eqb_spec x v); destruct (Var.eqb_spec x1 v); subst; simpl.
+    -- now contradiction H.
+    -- rewrite Var.eqb_refl; rewrite subst_closed_refl; auto; now rewrite <- Term.shift_closed_iff.
+    -- rewrite Var.eqb_refl; rewrite subst_closed_refl; auto; now rewrite <- Term.shift_closed_iff.
+    -- rewrite <- Var.eqb_neq in *; rewrite n; now rewrite n0.
+  - destruct (Var.eqb_spec x v); destruct (Var.eqb_spec x1 v); subst; simpl.
+    -- now contradiction H.
+    -- rewrite Var.eqb_refl; rewrite <- Var.eqb_neq in n; now rewrite n.
+    -- rewrite Var.eqb_refl; rewrite <- Var.eqb_neq in n; now rewrite n.
+    -- rewrite <- Var.eqb_neq in n,n0; rewrite n,n0; f_equal; now apply IHt.
+Qed.
+
+(** *** Substitution modulo shift function *)
+
+Lemma subst_shift_spec : forall lb k k' t x v,
+  <[[⧐ₜₘ lb ≤ k] ([x := v ~ lb ≤ k'] t)]> = 
+  <[[x := ([⧐ₜₘ lb ≤ k] v) ~ lb ≤ k'] ([⧐ₜₘ lb ≤ k] t)]>.
+Proof.
+  intros lb k k' t; revert lb k k'; induction t; intros lb k k' x v1; simpl;
+  f_equal; eauto.
+  - destruct (Var.eqb_spec x v); subst.
+    -- apply Term.shift_permute.
+    -- now simpl.
+  - destruct (Var.eqb x v); simpl; try reflexivity; f_equal; auto.
+Qed.
+
+Lemma subst_shift_spec_1 : forall lb k k' t x v,
+  <[[⧐ₜₘ lb ≤ k] ([x := v ~ lb ≤ k'] t)]> = 
+  <[[x := ([⧐ₜₘ lb ≤ k] v) ~ {lb + k} ≤ k'] ([⧐ₜₘ lb ≤ k] t)]>.
+Proof.
+  intros lb k k' t; revert lb k k'; induction t; intros lb k k' x v1; simpl;
+  f_equal; eauto.
+  - destruct (Var.eqb_spec x v); subst.
+    -- apply Term.shift_permute_1.
+    -- now simpl.
+  - destruct (Var.eqb x v); simpl; try reflexivity; f_equal; auto.
+Qed.
+
+Lemma subst_shift_spec_2 : forall lb lb' k k' t x v,
+  lb <= lb' ->
+  <[[⧐ₜₘ lb ≤ k] ([x := v ~ lb' ≤ k'] t)]> = 
+  <[[x := ([⧐ₜₘ lb ≤ k] v) ~ {lb' + k} ≤ k'] ([⧐ₜₘ lb ≤ k] t)]>.
+Proof.
+  intros lb lb' k k' t; revert lb lb' k k'; induction t; intros lb lb' k k' x v1 Hle; simpl;
+  f_equal; eauto.
+  - destruct (Var.eqb_spec x v); simpl; try reflexivity.
+    now apply Term.shift_permute_2.
+  - destruct (Var.eqb_spec x v); simpl; f_equal; auto.
+Qed.
+
+(** *** Valid through substitution *)
+
+Lemma subst_preserves_valid : forall k k' v x t,
+  k >= k' -> k ⊩ₜₘ t -> k' ⊩ₜₘ v -> k ⊩ₜₘ <[[x := v ~ k' ≤ {k - k'}] t]>.
+Proof.
+  intros k k' v x t; revert k k'; induction t; intros k k' Hle Hvt Hvv; auto;
+  try (unfold Term.valid in *; inversion Hvt; subst; constructor; now eauto).
+  - simpl; destruct (Var.eqb_spec x v0); subst; auto.
+    replace (k ⊩ₜₘ <[ [⧐ₜₘ k' ≤ {k - k'}] v ]>) 
+    with ((k' + (k - k')) ⊩ₜₘ <[ [⧐ₜₘ k' ≤ {k - k'}] v ]>).
+    -- now apply Term.shift_preserves_valid.
+    -- f_equal; lia.
+  - unfold Term.valid in *; inversion Hvt; subst; simpl. 
+    destruct (Var.eqb_spec x v0); subst; auto; constructor; auto.
+  - unfold Term.valid in *; inversion Hvt; subst; simpl; constructor;
+    auto. replace (S (S (k - k'))) with ((S (S k)) - k'); try lia. apply IHt2; auto.
+Qed.
+
+Lemma subst_preserves_valid_4 : forall k x v t,
+  k ⊩ₜₘ t ->  k ⊩ₜₘ v -> k ⊩ₜₘ <[[x := v ~ k] t]>.
+Proof.
+  intros k x v t Hvt; replace 0 with (k - k) by lia; apply subst_preserves_valid;
+  try assumption; lia.
+Qed.
+
+(** ** Evaluation Transition *)
+
+(** *** Lift semantics rules from evaluation to multi evaluation *)
+
+Lemma multi_var : forall k (x : variable), k ⊨ x ⟼⋆ x.
+Proof. intros k x; apply multi_refl. Qed.
+
+Lemma multi_appv : forall k x t τ v, 
+  value(v) -> k ⊨ ((\x:τ, t) v) ⟼⋆ ([x := v ~ k ≤ 0] t).
+Proof. 
+  intros k x t τ v Hv. apply multi_step with (y := <[[x := v ~ k ≤ 0] t]>); auto.
+Qed.
+
+Lemma multi_fix : forall k x t τ, 
+  k ⊨ (Fix (\x:τ, t)) ⟼⋆ ([x := (Fix (\x:τ, t)) ~ k ≤ 0] t).
+Proof. 
+  intros k x t τ. apply multi_step with (y := <[[x := (Fix (\x:τ, t)) ~ k ≤ 0] t]>); auto.
+Qed.
+
+Lemma multi_app1 : forall k t t' t2, k ⊨ t ⟼⋆ t' -> k ⊨ (t t2) ⟼⋆ (t' t2).
+Proof. 
+  intros k t t' t2 HeT; induction HeT; subst; auto.
+  apply multi_step with <[y t2]>; auto.
+Qed.
+
+Lemma multi_app2 : forall k t t' t1, value(t1) -> k ⊨ t ⟼⋆ t' -> k ⊨ (t1 t) ⟼⋆ (t1 t').
+Proof. 
+  intros k t t' t1 Hvt HeT; induction HeT; subst; auto.
+  apply multi_step with <[t1 y]>; auto.
+Qed.
+
+Lemma multi_pair1 : forall k t t' t2, k ⊨ t ⟼⋆ t' -> k ⊨ ⟨t,t2⟩ ⟼⋆ ⟨t',t2⟩.
+Proof.
+  intros k t t' t2 HeT; induction HeT; subst; auto.
+  apply multi_step with <[⟨y,t2⟩]>; auto. 
+Qed.
+
+Lemma multi_pair2 : forall k t t' t1, value(t1) -> k ⊨ t ⟼⋆ t' -> k ⊨ ⟨t1,t⟩ ⟼⋆ ⟨t1,t'⟩.
+Proof.
+  intros k t t' t1 Hvt HeT; induction HeT; subst; auto.
+  apply multi_step with <[⟨t1,y⟩]>; auto. 
+Qed.
+
+Lemma multi_fstv : forall k t1 t2, value(t1) -> value(t2) -> k ⊨ ⟨t1,t2⟩.fst ⟼⋆ t1.
+Proof.
+  intros k t1 t2 Hvt1 Hvt2; apply multi_step with t1; auto.
+Qed.
+
+Lemma multi_fst1 : forall k t t', k ⊨ t ⟼⋆ t' -> k ⊨ t.fst ⟼⋆ t'.fst.
+Proof.
+  intros k t t' HeT; induction HeT; subst; auto.
+  apply multi_step with <[y.fst]>; auto. 
+Qed.
+
+Lemma multi_sndv : forall k t1 t2, value(t1) -> value(t2) -> k ⊨ ⟨t1,t2⟩.snd ⟼⋆ t2.
+Proof.
+  intros k t1 t2 Hvt1 Hvt2; apply multi_step with t2; auto.
+Qed.
+
+Lemma multi_snd1 : forall k t t', k ⊨ t ⟼⋆ t' -> k ⊨ t.snd ⟼⋆ t'.snd.
+Proof.
+  intros k t t' HeT; induction HeT; subst; auto.
+  apply multi_step with <[y.snd]>; auto. 
+Qed.
+
+Lemma multi_arr : forall k t t', k ⊨ t ⟼⋆ t' -> k ⊨ arr(t) ⟼⋆ arr(t').
+Proof.
+  intros k t t' HeT; induction HeT; subst; auto.
+  apply multi_step with <[arr(y)]>; auto. 
+Qed.
+
+Lemma multi_first : forall k τ t t', k ⊨ t ⟼⋆ t' -> k ⊨ first(τ:t) ⟼⋆ first(τ:t').
+Proof.
+  intros k τ t t' HeT; induction HeT; subst; auto.
+  apply multi_step with <[first(τ:y)]>; auto. 
+Qed.
+
+Lemma multi_comp1 : forall k t t' t2, k ⊨ t ⟼⋆ t' -> k ⊨ t >>> t2 ⟼⋆ t' >>> t2.
+Proof. 
+  intros k t t' t2 HeT; induction HeT; subst; auto.
+  apply multi_step with <[y >>> t2]>; auto.
+Qed.
+
+Lemma multi_comp2 : forall k t t' t1, value(t1) -> k ⊨ t ⟼⋆ t' -> k ⊨ t1 >>> t ⟼⋆ t1 >>> t'.
+Proof. 
+  intros k t t' t1 Hvt HeT; induction HeT; subst; auto.
+  apply multi_step with <[t1 >>> y]>; auto.
+Qed.
+
+Lemma multi_wh1 : forall k t t' t2, k ⊨ t ⟼⋆ t' -> k ⊨ wormhole(t;t2) ⟼⋆ wormhole(t';t2).
+Proof. 
+  intros k t t' t2 HeT; induction HeT; subst; auto.
+  apply multi_step with <[wormhole(y;t2)]>; auto.
+Qed.
+
+Lemma multi_wh2 : forall k t t' t1, 
+  value(t1) -> (S (S k)) ⊨ t ⟼⋆ t' -> k ⊨ wormhole(t1;t) ⟼⋆ wormhole(t1;t').
+Proof. 
+  intros k t t' t1 Hvt HeT; dependent induction HeT; subst; auto.
+  apply multi_step with <[wormhole(t1;y)]>; auto.
+Qed.
+
+(** *** Value regards of evaluation transition *)
+
+Lemma value_normal : forall k t, value(t) -> normal_form k t.
+Proof.
+  intros k t H; generalize k; clear k; induction H; intros k [t' ST]; 
+  try (inversion ST; subst; try destruct (IHvalue k); now eauto);
+  try (inversion ST; subst; try destruct (IHvalue1 k); now eauto).
+  - destruct (IHvalue2 k). inversion ST; subst.
+    -- exfalso; apply (IHvalue1 k); now exists t1'.
+    -- now exists t'0.
+  - destruct (IHvalue2 k). inversion ST; subst.
+    -- exfalso; apply (IHvalue1 k); now exists t1'.
+    -- now exists t'0.
+  - destruct (IHvalue2 (S (S k))). inversion ST; subst.
+    -- exfalso; apply (IHvalue1 k); now exists i'.
+    -- now exists t'0.
+Qed.
+
+Lemma evaluate_not_value : forall t t' k, k ⊨ t ⟼ t' -> ~ (value(t)).
+Proof.
+  intros; induction H; unfold not; intro c; inversion c; subst; eauto.
+Qed.
+
+(** *** Transitivity of multiple evaluation steps *)
+
+Lemma multi_trans : forall k, Transitive (multi k).
+Proof.
+  red; intros k x y z HmeT HmeT'; induction HmeT; try assumption.
+  eapply multi_step; eauto.
+Qed.
+
+Lemma indexed_trans : forall lb k k' t t' t'',
+lb ⊨ t ⊢ k ⟶ t' -> lb ⊨ t' ⊢ k' ⟶ t'' -> lb ⊨ t ⊢ (k+k') ⟶ t''.
+Proof.
+  induction k; intros.
+  - simpl; inversion H; subst; auto.
+  - inversion H; subst. simpl. apply index_step with (y := y); auto.
+    eapply IHk; eauto.
+Qed.
+
+(** *** Valid *)
+
+Lemma evaluate_preserves_valid_term : forall t t' k,
+  k ⊩ₜₘ t -> k ⊨ t ⟼ t' -> k ⊩ₜₘ t'.
+Proof.
+  intros t; induction t; intros t' k Hvt HeTt; inversion Hvt; inversion HeTt; 
+  subst; auto; try (constructor; fold Term.valid in *; auto).
+  - inversion Hvt; subst; inversion H4; subst. now apply subst_preserves_valid_4.
+  - inversion Hvt; subst. inversion H5; subst; apply subst_preserves_valid_4; auto.
+  - inversion H1; subst; auto.
+  - inversion H1; subst; auto.
+Qed.
+
+Lemma multi_preserves_valid_term : forall k t t',
+  k ⊩ₜₘ t -> k ⊨ t ⟼⋆ t' -> k ⊩ₜₘ t'.
+Proof.
+  intros; induction H0; auto; apply IHmulti.
+  now apply evaluate_preserves_valid_term with (t := x).
+Qed.
+
+Lemma indexed_preserves_valid_term : forall n t t' k,
+  k ⊩ₜₘ t -> k ⊨ t ⊢ n ⟶ t' -> k ⊩ₜₘ t'.
+Proof.
+  intro n; induction n; intros t t' k Hvt Hi.
+  - inversion Hi; subst; assumption.
+  - inversion Hi; subst; apply IHn with (t := y); try assumption.
+    now apply evaluate_preserves_valid_term with (t := t).
+Qed. 
+
+Theorem evaluate_valid_weakening_gen : forall t t' lb lb' k k',
+  lb <= lb' -> k <= lb -> k' <= lb' -> k <= k' -> lb' - lb = k' - k ->
+  lb ⊨ t ⟼ t' -> lb' ⊨ ([⧐ₜₘ k ≤ {k' - k}] t) ⟼ ([⧐ₜₘ k ≤ {k' - k}] t').
+Proof.
+  intros t t' lb lb' k k' Hle1 Hle Hle' Hle2 Heq eT;
+  revert lb' k k' Hle Hle1 Hle2 Hle' Heq; induction eT; 
+  intros lb' k k' Hle Hle1 Hle2 Hle' Heq; simpl; eauto;
+  try (constructor; eauto; now apply Term.shift_value_iff).
+  - rewrite subst_shift_spec_2; auto. rewrite <- Heq. replace (lb + (lb' - lb)) with lb' by lia.
+    constructor; now apply Term.shift_value_iff.
+  - rewrite subst_shift_spec_2; auto. rewrite <- Heq. replace (lb + (lb' - lb)) with lb' by lia.
+    constructor.
+  - constructor; try (now rewrite <- Term.shift_value_iff); apply IHeT; lia.
+Qed.
+
+Theorem multi_evaluate_valid_weakening_gen : forall t t' lb lb' k k',
+  lb <= lb' -> k <= lb -> k' <= lb' -> k <= k' -> lb' - lb = k' - k ->
+  lb ⊨ t ⟼⋆ t' -> lb' ⊨ ([⧐ₜₘ k ≤ {k' - k}] t) ⟼⋆ ([⧐ₜₘ k ≤ {k' - k}] t').
+Proof.
+  intros; induction H4; try now constructor.
+  eapply multi_step with (y := <[[⧐ₜₘ k ≤ {k' - k}] y ]>); auto.
+  eapply evaluate_valid_weakening_gen with (lb := k0); auto.
+Qed.
+
+Theorem indexed_evaluate_valid_weakening_gen : forall t t' lb lb' k k' n,
+  lb <= lb' -> k <= lb -> k' <= lb' -> k <= k' -> lb' - lb = k' - k ->
+  lb ⊨ t ⊢ n ⟶ t' -> lb' ⊨ ([⧐ₜₘ k ≤ {k' - k}] t) ⊢ n ⟶ ([⧐ₜₘ k ≤ {k' - k}] t').
+Proof.
+  intros; induction H4; try now constructor.
+  eapply index_step with (y := <[[⧐ₜₘ k ≤ {k' - k}] y ]>); auto.
+  eapply evaluate_valid_weakening_gen with (lb := lb); auto.
+Qed.
+
+(** *** Determinism *)
+
+Theorem evaluate_deterministic : forall k t t1 t2,
+  k ⊨ t ⟼ t1 -> k ⊨ t ⟼ t2 -> t1 = t2.
+Proof with eauto.
+  intros k t t' t'' E1 E2; generalize dependent t''.
+  induction E1; intros t'' E2; inversion E2; subst; try (f_equal; now auto); 
+  exfalso; try (eapply value_normal; now eauto); clear E2...
+  - eapply value_normal in H...
+  - inversion E1; subst.
+    -- eapply value_normal in H0...
+    -- eapply value_normal in H2...
+  - inversion H3; subst.
+    -- eapply value_normal in H...
+    -- eapply value_normal in H0...
+  - inversion E1; subst.
+    -- eapply value_normal in H0...
+    -- eapply value_normal in H2...
+  - inversion H3; subst.
+    -- eapply value_normal in H...
+    -- eapply value_normal in H0...
+Qed.
+
+Theorem indexed_deterministic : forall n k t t1 t2,
+  k ⊨ t ⊢ n ⟶ t1 -> k ⊨ t ⊢ n ⟶ t2 -> t1 = t2.
+Proof.
+intros n; induction n; intros k t t1 t2 Hev1 Hev2.
+- inversion Hev1; inversion Hev2; subst; reflexivity.
+- inversion Hev1; inversion Hev2; subst.
+  apply evaluate_deterministic with (t1 := y) in H6; auto; subst. 
+  now apply IHn with (k := k) (t := y0).
+Qed.
+
+(** *** Halts *)
+
+Lemma value_halts : forall k t, value(t) -> halts k t.
+Proof. 
+  intros k t Hv; unfold halts; exists t; split; try assumption.
+  apply multi_refl.
+Qed.
+
+Lemma evaluate_preserves_halting : forall k t t',
+  k ⊨ t ⟼ t' -> (halts k t <-> halts k t').
+Proof.
+  intros k t t' HeT; unfold halts; split; intros [t'' [HmeT Hv]].
+  - destruct HmeT.
+    -- exfalso; apply (value_normal k) in Hv; unfold normal_form,not in Hv; apply Hv.
+      now exists t'.
+    -- apply (evaluate_deterministic k x t' y HeT) in H as Heq; subst.
+      exists z; split; assumption.
+  - exists t''; split; try assumption; now apply multi_step with (y := t').     
+Qed.
+
+Lemma multi_preserves_halting : forall k t t',
+  k ⊨ t ⟼⋆ t' -> (halts k t <-> halts k t').
+Proof.
+  intros k t t' HmeT; induction HmeT; unfold halts; split; intros [t'' [HmeT' Hv]];
+  try (exists t''; now split).
+  - apply evaluate_preserves_halting in H as H'.
+    assert (halts k x). { exists t''; now split. }
+    rewrite H' in H0; now rewrite IHHmeT in H0.
+  - apply evaluate_preserves_halting in H as H'.
+    assert (halts k z). { exists t''; now split. }
+    rewrite <- IHHmeT in H0. now rewrite <- H' in H0.
+Qed.
+
+Lemma halts_weakening : forall k k' t, k <= k' -> halts k t -> halts k' <[[⧐ₜₘ k ≤ {k' - k}] t]>.
+Proof.
+  unfold halts; intros. destruct H0 as [t' [HeT Hvt']].
+  exists <[[⧐ₜₘ k ≤ {k' - k}] t']>; split.
+  - eapply multi_evaluate_valid_weakening_gen; eauto.
+  - now apply Term.shift_value_iff.
+Qed.
+
+Lemma halts_weakening_1 : 
+  forall k k' t, halts k t -> halts (k + k') <[[⧐ₜₘ k ≤ k'] t]>.
+Proof.
+  intros. 
+  replace <[[⧐ₜₘ k ≤ k'] t]> with <[[⧐ₜₘ k ≤ {(k + k') - k}] t ]> by (f_equal; lia).
+  apply halts_weakening; auto; lia.
+Qed.
+
+Lemma halts_pair : forall k t1 t2,
+  halts k <[⟨t1,t2⟩]> <-> halts k t1 /\ halts k t2.
+Proof.
+  assert (Hpair : forall k t1 t2 t, k ⊨ ⟨t1,t2⟩ ⟼⋆ t -> exists t1' t2', t = <[⟨t1',t2'⟩]>).
+  {
+    intros k t1 t2 t HeT; dependent induction HeT; subst.
+    - exists t1; now exists t2.
+    - inversion H; subst; eauto. 
+  }
+  intros k t1 t2; split; intros HA.
+  - destruct HA as [t [HmeT Hvt]]. apply Hpair in HmeT as Heq.
+    destruct Heq as [t1' [t2' Heq]]; subst. dependent induction HmeT.
+    -- inversion Hvt; subst; split.
+       + exists t1'; split; auto.
+       + exists t2'; split; auto.
+    -- inversion H; subst.
+       + apply IHHmeT with (t1 := t1'0) (t2 := t2) in Hvt; auto.
+         destruct Hvt; split; auto; clear H1.
+         rewrite evaluate_preserves_halting; eauto.
+       + apply IHHmeT with (t1 := t1) (t2 := t') in Hvt; auto.
+         destruct Hvt; split; auto; clear H0.
+         rewrite evaluate_preserves_halting; eauto.
+  - destruct HA. destruct H as [t1' [HmeT1 Hvt1']];
+    destruct H0 as [t2' [HmeT2 Hvt2']].
+    exists <[⟨t1',t2'⟩]>; split.
+    -- apply multi_trans with <[⟨t1',t2⟩]>.
+       + now apply multi_pair1.
+       + now apply multi_pair2.
+    -- now constructor.
+Qed.
+
+Lemma halts_first : forall k τ t,
+  halts k <[first(τ:t)]> <-> halts k t.
+Proof.
+  intros k τ t; split; intros HA.
+  - destruct HA as [t' [HmeT Hvt]]; dependent induction HmeT.
+    -- inversion Hvt; subst; exists t; split; auto.
+    -- inversion H; subst. apply (IHHmeT τ t') in Hvt; eauto.
+       rewrite evaluate_preserves_halting; eauto.
+  - destruct HA as [t' [HmeT Hvt']]; exists <[first(τ:t')]>; split; auto.
+    now apply multi_first.
+Qed.
+
+Lemma halts_comp : forall k t1 t2,
+  halts k <[t1 >>> t2]> <-> halts k t1 /\ halts k t2.
+Proof.
+  assert (Hcomp : forall k t1 t2 t, k ⊨ t1 >>> t2 ⟼⋆ t ->
+                             exists t1' t2', t = <[t1' >>> t2']>).
+  {
+    intros k t1 t2 t HeT; dependent induction HeT; subst.
+    - exists t1; now exists t2.
+    - inversion H; subst; eauto. 
+  }
+  intros k t1 t2; split; intros HA.
+  - destruct HA as [t [HmeT Hvt]]. apply Hcomp in HmeT as Heq.
+    destruct Heq as [t1' [t2' Heq]]; subst. dependent induction HmeT.
+    -- inversion Hvt; subst; split.
+       + exists t1'; split; auto.
+       + exists t2'; split; auto.
+    -- inversion H; subst.
+       + apply IHHmeT with (t1 := t1'0) (t2 := t2) in Hvt; auto.
+         destruct Hvt; split; auto; clear H1.
+         rewrite evaluate_preserves_halting; eauto.
+       + apply IHHmeT with (t1 := t1) (t2 := t') in Hvt; auto.
+         destruct Hvt; split; auto; clear H0.
+         rewrite evaluate_preserves_halting; eauto.
+  - destruct HA. destruct H as [t1' [HmeT1 Hvt1']];
+    destruct H0 as [t2' [HmeT2 Hvt2']].
+    exists <[t1' >>> t2']>; split.
+    -- apply multi_trans with <[t1' >>> t2]>.
+       + now apply multi_comp1.
+       + now apply multi_comp2.
+    -- now constructor.
+Qed.
+
+Lemma halts_wh : forall k t1 t2,
+  halts k <[wormhole(t1;t2)]> <-> halts k t1 /\ halts (S (S k)) t2.
+Proof.
+  assert (Hwh : forall k t1 t2 t, k ⊨ wormhole(t1;t2) ⟼⋆ t ->
+                             exists t1' t2', t = <[wormhole(t1';t2')]>).
+  {
+    intros k t1 t2 t HeT; dependent induction HeT; subst.
+    - exists t1; now exists t2.
+    - inversion H; subst; eauto. 
+  }
+  intros k t1 t2; split; intros HA.
+  - destruct HA as [t [HmeT Hvt]]. apply Hwh in HmeT as Heq.
+    destruct Heq as [t1' [t2' Heq]]; subst. dependent induction HmeT.
+    -- inversion Hvt; subst; split.
+       + exists t1'; split; auto.
+       + exists t2'; split; auto.
+    -- inversion H; subst.
+       + apply IHHmeT with (t1 := i') (t2 := t2) in Hvt; auto.
+         destruct Hvt; split; auto; clear H1.
+         rewrite evaluate_preserves_halting; eauto.
+       + apply IHHmeT with (t1 := t1) (t2 := t') in Hvt; auto.
+         destruct Hvt; split; auto; clear H0.
+         rewrite evaluate_preserves_halting; eauto.
+  - destruct HA. destruct H as [t1' [HmeT1 Hvt1']];
+    destruct H0 as [t2' [HmeT2 Hvt2']].
+    exists <[wormhole(t1';t2')]>; split.
+    -- apply multi_trans with <[wormhole(t1';t2)]>.
+       + now apply multi_wh1.
+       + now apply multi_wh2.
+    -- now constructor.
+Qed.
+
+
+(** *** Relation between eval,multi and indexed transition *)
+
+Lemma evaluate_indexed_1_iff : forall k t t',
+  k ⊨ t ⟼ t' <-> k ⊨ t ⊢ 1 ⟶ t'.
+Proof.
+  split; intros.
+  - replace 1 with (0 + 1); eauto; 
+    eapply index_step; eauto; apply index_refl; auto.
+  - inversion H; subst. inversion H3; subst; auto.
+Qed.
+
+Lemma multi_indexed : forall lb t t',
+  lb ⊨ t ⟼⋆ t' -> exists k, lb ⊨ t ⊢ k ⟶ t'.
+Proof.
+  intros. induction H.
+  - exists 0. apply index_refl; auto.
+  - destruct IHmulti. exists (S x0). eapply index_step; eauto.
+Qed.
+
+
+(** *** Some corollaries *)  
+
+Corollary evaluate_valid_weakening : forall t t' k k',
+  k <= k' ->
+  k ⊨ t ⟼ t' -> k' ⊨ ([⧐ₜₘ k ≤ {k' - k}] t) ⟼ ([⧐ₜₘ k ≤ {k' - k}] t').
+Proof. intros. apply evaluate_valid_weakening_gen with (lb := k); eauto. Qed.
+
+Corollary multi_evaluate_valid_weakening : forall t t' k k',
+  k <= k' ->
+  k ⊨ t ⟼⋆ t' -> k' ⊨ ([⧐ₜₘ k ≤ {k' - k}] t) ⟼⋆ ([⧐ₜₘ k ≤ {k' - k}] t').
+Proof. intros; apply multi_evaluate_valid_weakening_gen with (lb := k); auto. Qed.
+
+Corollary indexed_evaluate_valid_weakening : forall t t' k k' n,
+  k <= k' ->
+  k ⊨ t ⊢ n ⟶ t' -> k' ⊨ ([⧐ₜₘ k ≤ {k' - k}] t) ⊢ n ⟶ ([⧐ₜₘ k ≤ {k' - k}] t').
+Proof. intros; apply indexed_evaluate_valid_weakening_gen with (lb := k); auto. Qed.
